\subsubsection{Comparison of Interpolants and Uniform Interpolants}

In this section we compare the Craig Interpolants obtained by Z3 and Mathsat for contradicting pairs of formulas and the uniform interpolant obtained by our implementation such
that the symbols to eliminate are the same
for each input problem for our implementation.

\begin{table}[h]
\centering
\begin{tabular}{ccc}
\toprule
\multicolumn{3}{c}{A-part: $f(z_1, v) = s_1 \land f(z_2, v) = s_2 \land f(f(y_1, v), f(y_2, v)) = t$} \\
\midrule 
{} & \multicolumn{2}{c}{B-parts} \\
\cmidrule{2-3} \\
{} & 
\makecell{$z_1 = z_2 \land z_2 = y_1$ \\ $\land z_2 = y_2 \land f(s_2, s_1) \neq t$} & 
\makecell{$z_1 = z_2 \land z_1 = y_1$ \\ $\land z_2 = y_2 \land f(s_1, s_2) \neq t$} \\
\midrule
\multirow{1}{*}{SMT Solvers} & \multicolumn{2}{c}{Interpolants} \\
\midrule
Z3 & 
\makecell{$((f(s_2, s_1) = t) \lor (\neg (z_2 = z_1))$ \\ $\lor ((\neg (s_1 = s_2)) \land ((s_2 = s_1) \lor$ \\ $(\neg (z_2 = z_1)))) \lor (\neg (y_1 = z_1))$ \\ $\lor (\neg (y_2 = z_1)))$} & 
\makecell{$((f(s_1, s_2) = t) \lor ((\neg (s_1 = s_2))$ \\ $\land ((s_2 = s_1) \lor (\neg (z_2 = z_1)))) \lor$ \\ $(\neg (z_2 = z_1)) \lor (\neg (y_1 = z_1))$ \\ $\lor (\neg (y_2 = z_1)))$} \\
\midrule
Mathsat & 
\makecell{$\neg ((\neg (t = f(s_2, s_1))) \land ((= z_2 y_1)$ \\ $\land ((= z_1 z_2) \land (= z_2 y_2))))$} & 
\makecell{$\neg ((\neg (t = f(s_1, s_2))) \land (((= z_1 z_2)$ \\ $ \land (= z_1 y_1)) \land (= z_1 y_2)))$}\\
\bottomrule
\end{tabular}
\end{table}

TODO: keep working here. Just mention that the output produced by our implementation is X and that X was stronger.

%%% Local Variables:
%%% mode: latex
%%% TeX-master: "main"
%%% End:
